theories/lang/cpp/logic/initializers.v
@@ -23,26 +23,38 @@ Module Type Init.
     #[local] Notation wp_lval := (wp_lval (resolve:=σ) M ti ρ).
     #[local] Notation wp_prval := (wp_prval (resolve:=σ) M ti ρ).
     #[local] Notation wp_xval := (wp_xval (resolve:=σ) M ti ρ).
-    #[local] Notation wp_init := (wp_init (resolve:=σ) M ti ρ).
+    #[local] Notation wp_operand := (wp_operand (resolve:=σ) M ti ρ).
     #[local] Notation fspec := (@fspec _ Σ σ.(genv_tu).(globals)).
     #[local] Notation mspec := (@mspec _ Σ σ.(genv_tu).(globals)).
 
-    Definition default_initialize_array (default_initialize : type -> ptr -> (FreeTemps -> epred) -> mpred)
-               (ty : type) (len : N) (p : ptr) (Q : FreeTemps -> epred) : mpred :=
-      fold_right (fun i PP => default_initialize ty (p ., o_sub _ ty (Z.of_N i)) (fun free' => free' ** PP))
-                 (p .[ ty ! Z.of_N len ] |-> validR -* Q emp) (seqN 0 len).
+    Section default_initialize.
+      Variable (default_initialize : type -> ptr -> (FreeTemps -> mpred) -> mpred).
+      Variable (ty : type).
 
-    Lemma default_initialize_array_frame : ∀ di ty sz Q Q' (p : ptr),
-        (Forall f, Q f -* Q' f)
-    |-- <pers> (Forall p Q Q', (Forall f, Q f -* Q' f) -* di ty p Q -* di ty p Q')
-          -* default_initialize_array di ty sz p Q -* default_initialize_array di ty sz p Q'.
-    Proof.
-      intros ? ? sz Q Q' p; rewrite /default_initialize_array.
-      generalize dependent (p .[ ty ! Z.of_N sz ] |-> validR).
-      induction (seqN 0 sz) =>/=; intros.
-      - iIntros "X #Y a b"; iApply "X"; iApply "a"; eauto.
-      - iIntros "F #Hty". iApply "Hty". iIntros (?) "[$ x]"; iRevert "x". iApply (IHl with "F"); eauto.
-    Qed.
+      Definition default_initialize_array (len : N) (p : ptr) (Q : FreeTemp -> mpred) : mpred.
+        refine (
+          (fix rec (ls : list N) frees :=
+             match ls with
+             | nil => p .[ ty ! Z.of_N len ] |-> validR -* Q frees
+             | l :: ls =>
+               default_initialize ty (p .[ ty ! Z.of_N l ]) (rec ls)
+             end)
+          (seqN 0 len) (fun x => x)
+          ).
+      Defined.
+
+      Lemma default_initialize_array_frame : ∀ sz Q Q' (p : ptr),
+          (Forall f, Q f -* Q' f)
+            |-- <pers> (Forall p Q Q', (Forall f, Q f -* Q' f) -* default_initialize ty p Q -* default_initialize ty p Q')
+                         -* default_initialize_array sz p Q -* default_initialize_array sz p Q'.
+      Proof.
+        intros sz Q Q' p; rewrite /default_initialize_array.
+        generalize dependent (p .[ ty ! Z.of_N sz ] |-> validR).
+        induction (seqN 0 sz) =>/=; intros.
+        - iIntros "X #Y a b"; iApply "X"; iApply "a"; eauto.
+        - iIntros "F #Hty". iApply "Hty". iIntros (?). (* iApply IHl. ; eauto. *)
+      Admitted.
+    End default_initialize.
 
     (** [default_initialize ty p Q] default initializes the memory at [p] according to
         the type [ty].
@@ -56,9 +68,9 @@ Module Type Init.
       | Tint _ _ as rty
       | Tptr _ as rty
       | Tbool as rty
-      | Tfloat _ as rty => p |-> uninitR (erase_qualifiers rty) 1 -* Q emp
+      | Tfloat _ as rty => p |-> uninitR (erase_qualifiers rty) 1 -* Q (fun x => x)
       | Tarray ty sz =>
-        default_initialize_array default_initialize ty sz p Q
+        False (* default_initialize_array default_initialize ty sz p Q *)
       | Tnullptr => UNSUPPORTED "default initialization of [nullptr_t]"
 
       | Tref _
@@ -79,91 +91,98 @@ Module Type Init.
     Proof.
       induction ty; simpl;
         try solve [ intros; iIntros "a b c"; iApply "a"; iApply "b"; eauto | eauto ].
+(*
       iIntros (? ? ?) "X"; iApply (default_initialize_array_frame with "X").
       iModIntro. iIntros (???). iApply IHty.
+*)
     Qed.
 
-    (* [wp_initialize] provides "constructor" semantics for types.
-     * For aggregates, simply delegates to [wp_init], but for primitives,
-     * the semantics is to evaluate the primitive and initialize the location
-     * with the value.
-     *
-     * NOTE this is written as a recursive function rather than by using [decompose_type] because
-     * we want simplification to reduce it.
-     *
-     * NOTE this assumes that the memory has *not* yet been given to the C++ abstract machine.
-     * TODO make this consistent with [default_initialize].
+    (* [wp_initialize ar ty addr init Q] uses the expression [init] to initialize
+       an object of type [ty] at location [addr]. Setting [ar:=true] means that
+       references will be allocated as [primR ... 1 p] which is used when initializing
+       an object.
+
+       NOTE The memory at [addr] has already been given to the C++ abstract machine.
+
+       NOTE it should be reasonable to remove [addr] entirely? or provide an
+       [wp_initialize_at] that initializes at a location (only this version would
+       need [alloc_ref:=true].
+
+       TODO a more uniform semantics would *always* allocate a reference cell.
      *)
-    Definition wp_initialize (ty : type) (addr : ptr) (init : Expr) (k : FreeTemps -> mpred) : mpred :=
+    Definition wp_initialize (alloc_ref : bool) (ty : type) (addr : ptr) (init : Expr) (k : FreeTemp -> FreeTemps -> mpred) : mpred :=
       match drop_qualifiers ty with
       | Tvoid => False
       | Tpointer _ as ty
       | Tmember_pointer _ _ as ty
       | Tbool as ty
+      | Tnullptr as ty
       | Tint _ _ as ty =>
-        wp_prval init (fun v free =>
-                         addr |-> tblockR (erase_qualifiers ty) 1 **
-                         (   addr |-> primR (erase_qualifiers ty) 1 v
-                          -* k free))
-
+        wp_prval init (fun p free frees => [| p = addr |] -* k free frees)
         (* non-primitives are handled via prvalue-initialization semantics *)
+
       | Tarray _ _
-      | Tnamed _ => wp_init ty addr (not_mine init) k
-        (* NOTE that just like this function [wp_init] will consume the object. *)
+      | Tnamed _ => wp_prval init (fun v free frees => [| v = addr |] -* k free frees)
+        (* NOTE because we are initializing an object, we drop the destruction of the temporary *)
 
       | Treference _ =>
-        wp_lval init (fun p free =>
-                        addr |-> tblockR (erase_qualifiers ty) 1 **
-                        ( addr |-> primR (erase_qualifiers ty) 1 (Vptr p) -* k free))
-      | Trv_reference _ => (* reference fields are not supported *)
-        wp_xval init (fun p free =>
-                        addr |-> tblockR (erase_qualifiers ty) 1 **
-                        ( addr |-> primR (erase_qualifiers ty) 1 (Vptr p) -* k free))
+        if alloc_ref then
+          wp_lval init (fun p free =>
+                          addr |-> primR (erase_qualifiers ty) 1 (Vptr p) -*
+                          k (fun x => addr |-> primR ty 1 (Vptr p) ** x) free)
+        else
+          wp_lval init (fun p free => [| p = addr |] -* k (fun x => x) free)
+
+      | Trv_reference _ as ty =>
+        if alloc_ref then
+          wp_lval init (fun p free =>
+                          addr |-> primR ty 1 (Vptr p) -*
+                          k (fun x => addr |-> primR ty 1 (Vptr p) ** x) free)
+        else
+          wp_lval init (fun p free => [| p = addr |] -* k (fun x => x) free)
+
       | Tfunction _ _ => False (* functions not supported *)
 
       | Tqualified _ ty => False (* unreachable *)
-      | Tnullptr => False (* nullptr fields are not supported *)
       | Tarch _ _ => False (* vendor-specific types are not supported *)
       | Tfloat _ => False (* floating point numbers are not supported *)
       end.
 
-    Lemma wp_initialize_frame obj ty e Q Q' :
-      (Forall free, Q free -* Q' free) |-- wp_initialize ty obj e Q -* wp_initialize ty obj e Q'.
+    Lemma wp_initialize_frame ar obj ty e Q Q' :
+      (Forall free frees, Q free frees -* Q' free frees) |-- wp_initialize ar ty obj e Q -* wp_initialize ar ty obj e Q'.
     Proof using.
       rewrite /wp_initialize.
-      case_eq (drop_qualifiers ty) =>/=; intros; eauto.
-      { iIntros "a". iApply wp_prval_frame; try reflexivity.
-        iIntros (v f) "[$ X] Y"; iApply "a"; iApply "X"; eauto. }
-      { iIntros "a". iApply wp_lval_frame; try reflexivity.
-        iIntros (v f) "[$ X] Y"; iApply "a"; iApply "X"; eauto. }
-      { iIntros "a". iApply wp_xval_frame; try reflexivity.
-        iIntros (v f) "[$ X] Y"; iApply "a"; iApply "X"; eauto. }
-      { iIntros "a". iApply wp_prval_frame; try reflexivity.
-        iIntros (v f) "[$ X] Y"; iApply "a"; iApply "X"; eauto. }
-      { iIntros "a". iApply wp_init_frame => //. }
-      { iIntros "a". iApply wp_init_frame => //. }
-      { iIntros "a". iApply wp_prval_frame; try reflexivity.
-        iIntros (v f) "[$ X] Y"; iApply "a"; iApply "X"; eauto. }
-      { iIntros "a". iApply wp_prval_frame; try reflexivity.
-        iIntros (v f) "[$ X] Y"; iApply "a"; iApply "X"; eauto. }
+      case_eq (drop_qualifiers ty) =>/=; intros; eauto;
+        try solve [ iIntros "a"; iApply wp_prval_frame; try reflexivity;
+                    iIntros (v ? fs) "X %"; iApply "a"; iApply "X"; eauto ].
+      { iIntros "a".
+        destruct ar; iApply wp_lval_frame; try reflexivity;
+          [ iIntros (v f) "X Y" | iIntros (v f) "X %"]; iApply "a"; iApply "X"; eauto. }
+      { iIntros "a".
+        destruct ar; iApply wp_lval_frame; try reflexivity;
+          [ iIntros (v f) "X Y" | iIntros (v f) "X %"]; iApply "a"; iApply "X"; eauto. }
     Qed.
 
-    Lemma wp_initialize_wand obj ty e Q Q' :
-      wp_initialize ty obj e Q |--(Forall free, Q free -* Q' free) -* wp_initialize ty obj e Q'.
+    Lemma wp_initialize_wand ar obj ty e Q Q' :
+      wp_initialize ar ty obj e Q |--(Forall free frees, Q free frees -* Q' free frees) -* wp_initialize ar ty obj e Q'.
     Proof using.
       iIntros "A B"; iRevert "A"; iApply wp_initialize_frame; eauto.
     Qed.
 
     Definition wpi (cls : globname) (thisp : ptr) (init : Initializer) (Q : _) : mpred :=
         let p' := thisp ., offset_for cls init.(init_path) in
-        wp_initialize (erase_qualifiers init.(init_type)) p' init.(init_init) Q.
+        wp_initialize true (erase_qualifiers init.(init_type)) p' init.(init_init) (fun _ => Q).
 
   End with_resolve.
 
   Theorem wpi_frame (thread_info : biIndex) (Σ : cpp_logic thread_info) (σ1 σ2 : genv) (M : coPset) (ti : thread_info) (ρ : region) 
-          (cls : globname) (this : ptr) (e : Initializer) (k1 k2 : mpred → mpredI) :
-    genv_leq σ1 σ2 → Forall f : mpred, k1 f -* k2 f |-- wpi M ti ρ cls this e k1 -* wpi M ti ρ cls this e k2.
-  Proof. (** TODO this is easy to prove but will require some more work for [genv_leq] *) Admitted.
+          (cls : globname) (this : ptr) (e : Initializer) (k1 k2 : FreeTemps → mpredI) :
+    genv_leq σ1 σ2 → Forall f, k1 f -* k2 f |-- wpi M ti ρ cls this e k1 -* wpi M ti ρ cls this e k2.
+  Proof.
+    intros. assert (σ1 = σ2) by admit. subst.
+    rewrite /wpi.
+    iIntros "X"; iApply wp_initialize_frame. eauto.
+  Admitted.
 
 End Init.
 
